src/Parsers/ParserFromParserADT.v
@@ -28,7 +28,7 @@ Section parser.
   Context {stringlike_stringlikemin : StringLikeMin Ascii.ascii}
           {stringlike_stringlike : StringLike Ascii.ascii}
           {stringlike_stringlike_properties : StringLikeProperties Ascii.ascii}.
-  Context {G : pregrammar' Ascii.ascii}.
+  Context {G : pregrammar Ascii.ascii}.
   Context (Hvalid : is_true (grammar_rvalid G)).
   Context (splitter_impl : FullySharpened (string_spec G stringlike_stringlike)).
 
@@ -126,41 +126,42 @@ Module Import local_opt.
   Ltac change_opt' ls nt str :=
     idtac;
     match goal with
-      | _ => progress change (List.map fst ls) with (opt.map opt.fst ls)
-      | _ => progress change (snd (of_string str)) with (opt.snd (of_string str))
-      | _ => progress change (Equality.string_beq nt) with (opt.string_beq nt)
+      | _ => progress change (List.map fst ls) with (opt.id (opt.map opt.fst ls))
+      | _ => progress change (List.length ls) with (opt.id (opt.length ls))
+      | _ => progress change (snd (of_string str)) with (opt.id (opt.snd (of_string str)))
+      | _ => progress change (Equality.string_beq nt) with (opt.id (opt.string_beq nt))
       | _ => progress change (Operations.List.uniquize (fun x0 y0 => Equality.string_beq (fst x0) (fst y0)) ls)
-             with (opt.uniquize (fun x0 y0 => opt.string_beq (opt.fst x0) (opt.fst y0)) ls)
-      | [ |- context G[Operations.List.uniquize Equality.string_beq (opt.map ?f ?ls)] ]
-        => progress change (Operations.List.uniquize Equality.string_beq (opt.map f ls))
-           with (opt.uniquize opt.string_beq (opt.map f ls))
-      | [ |- context G[List.length (opt.uniquize ?beq ?ls)] ]
-        => progress change (List.length (opt.uniquize beq ls))
-           with (opt.length (opt.uniquize beq ls))
-      | [ |- context G[Operations.List.first_index_default (opt.string_beq ?x) (opt.length ?ls) (opt.uniquize ?beq ?ls')] ]
-        => change (Operations.List.first_index_default (opt.string_beq x) (opt.length ls) (opt.uniquize beq ls'))
-           with (opt.first_index_default (opt.string_beq x) (opt.length ls) (opt.uniquize beq ls'))
-      | [ |- context G[Operations.List.up_to (opt.length ?ls)] ]
-        => change (Operations.List.up_to (opt.length ls))
-           with (opt.up_to (opt.length ls))
-      | [ |- context G[List.rev (opt.up_to ?ls)] ]
-        => change (List.rev (opt.up_to ls))
-           with (opt.rev (opt.up_to ls))
+             with (opt.id (opt.uniquize (fun x0 y0 => opt.string_beq (opt.fst x0) (opt.fst y0)) ls))
+      | [ |- context G[Operations.List.uniquize Equality.string_beq (opt.id ?ls)] ]
+        => progress change (Operations.List.uniquize Equality.string_beq (opt.id ls))
+           with (opt.uniquize opt.string_beq ls)
+      | [ |- context G[List.length (opt.id ?ls)] ]
+        => progress change (List.length (opt.id ls))
+           with (opt.id (opt.length ls))
+      | [ |- context G[Operations.List.first_index_default (opt.id ?beq) (opt.id ?len) (opt.id ?ls)] ]
+        => change (Operations.List.first_index_default (opt.id beq) (opt.id len) (opt.id ls))
+           with (opt.id (opt.first_index_default beq len ls))
+      | [ |- context G[Operations.List.up_to (opt.id ?n)] ]
+        => change (Operations.List.up_to (opt.id n))
+           with (opt.id (opt.up_to n))
+      | [ |- context G[List.rev (opt.id ?ls)] ]
+        => change (List.rev (opt.id ls))
+           with (opt.id (opt.rev ls))
       | [ |- context G[List.map (fun x0 : ?T => Operations.List.up_to (Datatypes.length (snd x0)))
-                                (opt.uniquize ?beq ?ls)] ]
+                                (opt.id ?ls)] ]
         => change (List.map (fun x0 : T => Operations.List.up_to (Datatypes.length (snd x0)))
-                            (opt.uniquize beq ls))
-           with (opt.map (fun x0 : T => opt.up_to (opt.length (snd x0)))
-                         (opt.uniquize beq ls))
-      | [ |- context G[List.combine (opt.rev ?ls) (opt.map ?f ?ls')] ]
-        => change (List.combine (opt.rev ls) (opt.map f ls'))
-           with (opt.combine (opt.rev ls) (opt.map f ls'))
-      | [ |- context G[snd (pcMethods ?x ?y ?z ?w ?v)] ]
-        => change (snd (pcMethods x y z w v))
-           with (opt.snd (pcMethods x y z w v))
-      | [ |- context G[List.hd ?d (opt.uniquize ?beq ?ls)] ]
-        => change (List.hd d (opt.uniquize beq ls))
-           with (opt.hd d (opt.uniquize beq ls))
+                            (opt.id ls))
+           with (opt.id (opt.map (fun x0 : T => opt.up_to (opt.length (snd x0)))
+                                 ls))
+      | [ |- context G[List.combine (opt.id ?ls) (opt.id ?ls')] ]
+        => change (List.combine (opt.id ls) (opt.id ls'))
+           with (opt.id (opt.combine ls ls'))
+      | [ |- context G[snd (pcMethods ?x ?y ?z)] ]
+        => change (snd (pcMethods x y z))
+           with (opt.id (opt.snd (pcMethods x y z)))
+      | [ |- context G[List.hd ?d (opt.id ?ls)] ]
+        => change (List.hd d (opt.id ls))
+           with (opt.id (opt.hd d ls))
     end.
 
   Ltac change_opt ls nt str := repeat change_opt' ls nt str.
@@ -181,43 +182,78 @@ Local Ltac do_change_snd h impl :=
   let v := (eval cbv beta in v) in
   change term with v; cbv beta.
 
+Local Ltac replace_rewrite_map_map :=
+  idtac;
+  let RHS := match goal with |- _ = ?RHS => RHS end in
+  let LHS := match goal with |- ?LHS = _ => LHS end in
+  match RHS with
+  | context G[@List.map ?B ?C ?g (@List.map ?A ?B ?f ?ls)]
+    => let x := fresh in
+       let y := fresh in
+       pose (@List.map B C g (@List.map A B f ls)) as x;
+       pose (@List.map A C (fun x => g (f x)) ls) as y;
+       let G' := context G[x] in
+       change (LHS = G');
+       replace x with y by (subst x y; symmetry; apply List.map_map);
+       subst x y
+  end.
+Local Ltac replace_rewrite_map_length :=
+  idtac;
+  let RHS := match goal with |- _ = ?RHS => RHS end in
+  let LHS := match goal with |- ?LHS = _ => LHS end in
+  match RHS with
+  | context G[@List.length ?B (@List.map ?A ?B ?f ?ls)]
+    => let x := fresh in
+       let y := fresh in
+       pose (@List.length B (@List.map A B f ls)) as x;
+       pose (@List.length A ls) as y;
+       let G' := context G[x] in
+       change (LHS = G');
+       replace x with y by (subst x y; symmetry; apply List.map_length);
+       subst x y
+  end.
+
 Definition parser
            {HSLM : StringLikeMin Ascii.ascii}
            {HSL : StringLike Ascii.ascii}
            {HSLP : StringLikeProperties Ascii.ascii}
-           {G : pregrammar' Ascii.ascii}
+           {G : pregrammar Ascii.ascii}
            (Hvalid : is_true (grammar_rvalid G))
            (splitter_impl : FullySharpened (string_spec G HSL))
 : Parser G HSL.
 Proof.
   let term := (eval cbv beta delta [parser''] in (@parser'' HSLM HSL HSLP G Hvalid splitter_impl)) in
   refine (term _ _ _ _);
-    cbv beta iota zeta delta [split_dataProj' has_parse parse parser' pdata' ParserImplementation.parser_data parser' parser transfer_parser RDPList.rdp_list_predata new_string_of_string proj adtProj proj1_sig new_string_of_base_string cConstructors StringLike.length adt_based_StringLikeMin adt_based_StringLikeMin_lite adt_based_StringLike_lite pdata BaseTypes.split_string_for_production split_dataProj adt_based_splitter BuildComputationalADT.callcADTMethod ibound indexb cMethods cRep BaseTypes.predata ParserImplementation.parser_data adt_based_StringLike RDPList.rdp_list_predata RDPList.rdp_list_nonterminals_listT list_to_grammar Valid_nonterminals RDPList.rdp_list_is_valid_nonterminal RDPList.rdp_list_remove_nonterminal string_type_min list_to_productions newS Fin.R mto_string msplits drop take is_char String length get bool_eq beq mlength mchar_at_matches mdrop mtake mget RDPList.rdp_list_initial_nonterminals_data default_nonterminal_carrierT production_carrierT default_production_carrierT char_at_matches unsafe_get RDPList.rdp_list_of_nonterminal production_tl split_data to_production RDPList.rdp_list_nonterminal_to_production ParserImplementation.parser_split_data RecognizerPreOptimized.optsplitdata RDPList.rdp_list_production_tl default_production_tl split_string_for_production RDPList.rdp_list_to_production RDPList.rdp_list_to_nonterminal Lookup grammar_of_pregrammar pregrammar'_of_pregrammar default_to_nonterminal default_to_production splits_for Lookup_idx Lookup_string];
-    change_opt (pregrammar_productions G) nt str.
+    cbv beta iota zeta delta [split_dataProj' has_parse parse parser' pdata' ParserImplementation.parser_data parser' parser transfer_parser];
+    progress repeat replace_rewrite_map_map; simpl @fst;
+      progress repeat replace_rewrite_map_length;
+      change (fun x : ?A * ?B => fst x) with (@fst A B);
+      cbv [split_dataProj' has_parse parse parser' pdata' ParserImplementation.parser_data parser' parser transfer_parser RDPList.rdp_list_predata new_string_of_string proj adtProj proj1_sig new_string_of_base_string cConstructors StringLike.length adt_based_StringLikeMin adt_based_StringLikeMin_lite adt_based_StringLike_lite pdata BaseTypes.split_string_for_production split_dataProj adt_based_splitter BuildComputationalADT.callcADTMethod ibound indexb cMethods cRep BaseTypes.predata ParserImplementation.parser_data adt_based_StringLike RDPList.rdp_list_predata RDPList.rdp_list_nonterminals_listT list_to_grammar Valid_nonterminals RDPList.rdp_list_is_valid_nonterminal RDPList.rdp_list_remove_nonterminal string_type_min list_to_productions newS Fin.R mto_string msplits drop take is_char String length get bool_eq beq mlength mchar_at_matches mdrop mtake mget RDPList.rdp_list_initial_nonterminals_data default_nonterminal_carrierT production_carrierT default_production_carrierT char_at_matches unsafe_get RDPList.rdp_list_of_nonterminal production_tl split_data to_production RDPList.rdp_list_nonterminal_to_production ParserImplementation.parser_split_data RecognizerPreOptimized.optsplitdata RDPList.rdp_list_production_tl default_production_tl split_string_for_production RDPList.rdp_list_to_production RDPList.rdp_list_to_nonterminal Lookup grammar_of_pregrammar pregrammar'_of_pregrammar default_to_nonterminal default_to_production splits_for Lookup_idx Lookup_string pregrammar_productions];
+    change_opt (pregrammar_rproductions G) nt str.
   { lazymatch goal with
     | [ |- appcontext[BooleanRecognizerOptimized.opt.opt.id
                         (BooleanRecognizerOptimized.opt.opt.first_index_default
                            ?a ?b
                            (BooleanRecognizerOptimized.opt.opt.map
-                              BooleanRecognizerOptimized.opt.opt.fst (pregrammar_productions G)))] ]
+                              BooleanRecognizerOptimized.opt.opt.fst (pregrammar_rproductions G)))] ]
       => replace (BooleanRecognizerOptimized.opt.opt.id
                     (BooleanRecognizerOptimized.opt.opt.first_index_default
                        a
                        b
                        (BooleanRecognizerOptimized.opt.opt.map
-                          BooleanRecognizerOptimized.opt.opt.fst (pregrammar_productions G))))
+                          BooleanRecognizerOptimized.opt.opt.fst (pregrammar_rproductions G))))
          with (BooleanRecognizerOptimized.opt.opt.list_caset
                  (fun _ => _)
                  b
                  (fun _ _ => 0)
-                 (pregrammar_productions G))
+                 (pregrammar_rproductions G))
     end.
     { match goal with
       | [ |- _ = ?x :> ?T ] => instantiate (1 := x); exact_no_check (@eq_refl T x)
       end. }
     { abstract (
           clear;
-          destruct (pregrammar_productions G); unfold BooleanRecognizerOptimized.opt.opt.first_index_default, BooleanRecognizerOptimized.opt.opt.id; simpl;
+          destruct (pregrammar_rproductions G); unfold BooleanRecognizerOptimized.opt.opt.first_index_default, BooleanRecognizerOptimized.opt.opt.id; simpl;
           [ reflexivity | ];
           change @BooleanRecognizerOptimized.opt.opt.string_beq with Equality.string_beq;
           rewrite Equality.string_lb by reflexivity;
